memory_props/MemoryProps2.ec
@@ -1,0 +1,355 @@
+require import AllCore Distr DBool.
+
+
+
+require import Reflection ReflectionComp.
+
+clone import ReflComp with type at1 <- unit,
+                           type at2 <- unit,
+                           type rt1 <- unit.
+
+
+
+
+section.
+declare module A <: RewEx1Ex2.
+axiom A_run_ll : islossless A.ex1.    
+lemma  qq &m : phoare[ A.ex1 :  (glob A) = (glob A){m} ==> exists &n, (glob A) = (glob A){n} ]=  1%r.
+proc*.
+seq 1 : true. auto.
+call A_run_ll. auto. skip.
+progress. exists &hr. auto.
+hoare. auto. auto.   
+qed.
+
+lemma rl  &m : Pr[ A.ex1() @ &m : exists &n, (glob A) = (glob A){n} ] =  1%r.
+byphoare (_: (glob A) = (glob A){m} ==> _). apply (qq &m). auto. auto.
+qed.
+
+
+
+
+
+
+require import RandomFacts RealSeries List.
+
+axiom ler_trans1 (a b c : real) : a <= b => b < c => a < c.
+
+lemma www &m p :   
+    exists (D1 : unit -> (glob A) -> (unit * (glob A)) distr)
+      (D2 : unit -> unit * (glob A) -> (glob A) Distr.distr),
+      (forall &m (M : unit * (glob A) -> bool),
+         mu (D1 tt (glob A){m}) M = Pr[A.ex1() @ &m : M (res, (glob A))]) /\
+      (forall &m (M : (glob A) -> bool) (r1 i2 : unit),
+         mu (D2 i2 (r1, (glob A){m})) M =
+         Pr[A.ex2(i2, r1) @ &m : M (glob A)]) /\
+      (forall &m (M : (glob A) -> bool) (i1 i2 : unit),
+        mu ((dlet (D1 i1 (glob A){m}) (D2 i2))) M =
+        Pr[RCR(A).main(i1, i2) @ &m : M (glob A)]) 
+   /\ forall (M :  (glob A) -> bool), 
+       p >= Pr[ RCR(A).main(tt,tt) @ &m : M (glob A) ]  =>
+       0%r < p =>
+   exists g, 0%r < mu1 (D1 tt (glob A){m}) (tt,g)  /\ mu (D2 tt ((tt,g))) M <= p.
+proof.  elim (refl_comp_simple A). progress.
+exists D1 D2. progress. rewrite H. auto.
+pose g0 := (glob A){m}.
+case (exists (g : (glob A)),
+  0%r < mu1 (D1 tt g0) (tt, g) /\ p >= mu (D2 tt (tt, g)) M).
+auto.
+move => G.
+have: (forall (g : (glob A)),
+     ! (0%r < mu1 (D1 tt g0) (tt, g) /\ p >= mu (D2 tt (tt, g)) M)).
+smt.
+clear G.
+move => G.
+have q : forall (g : glob A),  mu1 (D1 tt g0) (tt,g) > 0%r => mu (D2 tt (tt,g)) M > p .
+smt.
+have q2 : exists g, 0%r < mu1 (D1 tt g0) (tt, g).
+case (exists (g : (glob A)), 0%r < mu1 (D1 tt g0) (tt, g)). auto.
+move => q21.
+have q22  : forall (g : (glob A)), 0%r = mu1 (D1 tt g0) (tt, g).
+smt. clear q21.
+have : Pr[RCR(A).main(tt, tt) @ &m : true ] = 0%r.
+rewrite -  (H1 &m predT). 
+rewrite dlet_mu_main. 
+apply sum0_eq. progress. 
+ have -> : x = (tt, x.`2). smt.
+rewrite - q22. smt. admit.
+elim q2. move => g gp.
+have : mu (dlet (D1 tt (glob A){m}) (D2 tt)) M > p.
+rewrite  dlet_mu_main.
+rewrite (sum_split _ (pred1 (tt, g))). 
+apply (summable_mu1_wght ((D1 tt (glob A){m})) (fun x => mu (D2 tt x) M)   _) .
+smt.
+simplify.
+have -> : sum
+  (fun (x : unit * (glob A)) =>
+     if  pred1 (tt, g) x then mu1 (D1 tt (glob A){m}) x * mu (D2 tt x) M
+     else 0%r) = mu1 (D1 tt (glob A){m}) (tt,g) * mu (D2 tt (tt,g)) M.
+  have ->: (fun (x : unit * (glob A)) =>
+     if  pred1 (tt, g) x then mu1 (D1 tt (glob A){m}) x * mu (D2 tt x) M
+     else 0%r) = (fun (x : unit * (glob A)) => mu1 (D1 tt (glob A){m}) (tt,g) * mu (D2 tt (tt,g)) M *
+     if  pred1 (tt, g) x then (mu1 (duniform [(tt,g)]) x)
+     else 0%r).
+apply fun_ext. move => x.  
+case (pred1 (tt, g) x). simplify. progress.
+rewrite H4. 
+have -> : mu1 (duniform [(tt, g)]) (tt, g) = 1%r. smt. smt.
+smt.
+rewrite sumZ. 
+rewrite - muE. progress.
+have ->: mu1 (duniform [(tt, g)]) (tt, g) = 1%r. smt. smt.
+have zzz : sum
+  (fun (x : unit * (glob A)) =>
+     if ! pred1 (tt, g) x then mu1 (D1 tt (glob A){m}) x * mu (D2 tt x) M
+     else 0%r) >= sum
+  (fun (x : unit * (glob A)) =>
+     if ! pred1 (tt, g) x then mu1 (D1 tt (glob A){m}) x * p
+     else 0%r).
+apply ler_sum. progress. 
+case (pred1 (tt, g) x). simplify. auto. simplify. progress.
+have ->: x = (tt,x.`2). smt.
+case (mu1 (D1 tt (glob A){m}) (tt, x.`2) = 0%r). 
+smt. clear H4 G  H2 H1 H0 H . progress.
+have : p <= mu (D2 tt (tt, x.`2)) M. smt. progress. 
+have : 0%r < mu1 (D1 tt (glob A){m}) (tt, x.`2) . smt.
+smt.
+have ->: (fun (x : unit * (glob A)) =>
+     if ! pred1 (tt, g) x then mu1 (D1 tt (glob A){m}) x * p
+     else 0%r) = (fun (x : unit * (glob A)) => mu1 (D1 tt (glob A){m}) x * 
+     if ! pred1 (tt, g) x then p
+     else 0%r).
+apply fun_ext. move => x. smt.
+apply summable_mu1_wght. progress. smt. smt.
+have -> : (fun (x : unit * (glob A)) =>
+     if ! pred1 (tt, g) x then mu1 (D1 tt (glob A){m}) x *  mu (D2 tt x) M else 0%r)
+ = (fun (x : unit * (glob A)) =>  mu (D2 tt x) M *
+     if ! pred1 (tt, g) x then mu1 (D1 tt (glob A){m}) x else 0%r).
+apply fun_ext. move => x. smt. 
+
+have ->: (fun (x : unit * (glob A)) =>
+     mu (D2 tt x) M *
+     if ! pred1 (tt, g) x then mu1 (D1 tt (glob A){m}) x else 0%r)
+
+ = (fun (x : unit * (glob A)) =>
+     mu1 (D1 tt (glob A){m}) x *
+     if ! pred1 (tt, g) x then  mu (D2 tt x) M else 0%r).
+ apply fun_ext. move => zz. smt. 
+ apply summable_mu1_wght. progress. smt. smt. 
+have : mu1 (D1 tt (glob A){m}) (tt, g) * mu (D2 tt (tt, g)) M +
+sum
+  (fun (x : unit * (glob A)) =>
+     if ! pred1 (tt, g) x then mu1 (D1 tt (glob A){m}) x * p
+     else 0%r) > p.
+
+
+apply (ler_trans1 p (mu1 (D1 tt (glob A){m}) (tt, g) * p +
+sum
+  (fun (x : unit * (glob A)) =>
+          if ! pred1 (tt, g) x then mu1 (D1 tt (glob A){m}) x * p else 0%r) )   _ _).
+clear zzz G H H0 H1.
+have : mu (D2 tt (tt, g)) M
+ >  p.
+smt. progress.  
+have ->: mu1 (D1 tt (glob A){m}) (tt, g) * p +
+ sum
+  (fun (x : unit * (glob A)) =>
+     if ! pred1 (tt, g) x then mu1 (D1 tt (glob A){m}) x * p else 0%r)
+  = sum
+  (fun (x : unit * (glob A)) =>
+      mu1 (D1 tt (glob A){m}) x * p).
+rewrite (sumD1 (fun (x : unit * (glob A)) => mu1 (D1 tt (glob A){m}) x * p) (tt,g)). 
+have ->: (fun (x : unit * (glob A)) => mu1 (D1 tt (glob A){m}) x * p) 
+ = (fun (x : unit * (glob A)) => p * mu1 (D1 tt (glob A){m}) x ).
+smt.
+apply summableZ.
+apply summable_mu1.
+simplify. auto.
+
+
+have ->: sum (fun (x : unit * (glob A)) => mu1 (D1 tt (glob A){m}) x * p)
+ = p * sum (fun (x : unit * (glob A)) => mu1 (D1 tt (glob A){m}) x).
+rewrite -  sumZ.   simplify.
+ have ->: (fun (x : unit * (glob A)) => mu1 (D1 tt (glob A){m}) x * p) 
+ = (fun (x : unit * (glob A)) => p * mu1 (D1 tt (glob A){m}) x).
+smt.
+auto.
+have ->: (fun (x : unit * (glob A)) => mu1 (D1 tt (glob A){m}) x)
+ = (fun (x : unit * (glob A)) => if predT x then mu1 (D1 tt (glob A){m}) x else 0%r).
+smt.
+rewrite - muE.  
+have ->: weight (D1 tt (glob A){m}) = 1%r. admit. smt.
+
+
+
+have : mu (D2 tt (tt, g)) M
+ >  p.
+smt. smt.
+smt.
+
+
+
+rewrite H1. smt.
+qed.
+
+
+
+
+lemma ZzZ &m M i1 i2 p: 
+       p >= Pr[ RCR(A).main(i1,i2) @ &m : M (glob A) ] 
+   => 0%r < p
+   => exists &n, p >= Pr[ A.ex2(tt, tt) @ &n  : M (glob A)] .
+elim (www &m p). progress.
+elim (H2 M _ _);auto. smt. progress.
+have f1 : Pr[A.ex1() @ &m : glob A = g] > 0%r.
+have f2 : mu (D1 tt (glob A){m}) (fun x => snd x = g)  = Pr[A.ex1() @ &m : (glob A) = g].
+rewrite (H &m ). auto. smt. 
+have f3: exists &n, g = (glob A){n}.
+  have  f31: Pr[A.ex1() @ &m : (glob A) = g /\ (exists &n, (glob A) = (glob A){n}) ] = Pr[A.ex1() @ &m : (glob A) = g].
+  have <- : Pr[A.ex1() @ &m : (glob A) = g] = Pr[A.ex1() @ &m : (glob A) = g /\ exists &n, (glob A) = (glob A){n}].
+  rewrite Pr[mu_split exists &n, (glob A) = (glob A){n}].
+  have : Pr[A.ex1() @ &m : (glob A) = g /\ ! (exists &n, (glob A) = (glob A){n})] = 0%r. smt. smt. auto.
+  have f32 : Pr[A.ex1() @ &m : (glob A) = g /\ exists &n, g = (glob A){n}] =
+     Pr[A.ex1() @ &m : (glob A) = g].
+  rewrite - f31. rewrite Pr[mu_eq]. progress. auto.
+  have f33 : Pr[A.ex1() @ &m : exists &n, g = (glob A){n}] > 0%r.
+         have f331 : Pr[A.ex1() @ &m : (glob A) = g /\ exists &n, (glob A) = (glob A){n}] 
+                         >= Pr[A.ex1() @ &m : (glob A) = g]. smt.
+       smt.
+  clear f32 f31 f1    H2 H1 H0 H. 
+  case (exists &n, g = (glob A){n}). auto.
+  move => q. 
+   have : Pr[A.ex1() @ &m : exists &n, g = (glob A){n}] = Pr[A.ex1() @ &m : false]. 
+   rewrite Pr[mu_eq]. progress. auto. smt.
+elim f3. progress.
+exists &n.
+rewrite -  (H0 &n M tt tt). auto.
+qed.
+
+
+
+module type IR1R2 = {
+  proc init() : unit
+  proc run1() : bool
+  proc run2() : bool
+}.
+
+module P(A : IR1R2) = {
+  proc main1() = {
+    var r : bool;
+    A.init();
+    r <@ A.run1();
+    return r;
+  }
+
+  proc main2() = {
+    var r : bool;
+    A.init();
+    r <@ A.run2();
+    return r;
+  }
+
+  proc init_main12() = {
+   var b, r', r : bool;
+
+   A.init();
+   b <$ {0,1};
+   
+   if(b){
+     r <@ A.run1();
+   }else{
+     r' <@ A.run2();
+     r  <- !r;
+   }
+   return r;
+  }
+
+  proc main12() = {
+   var b, r', r : bool;
+   b <$ {0,1};
+   
+   if(b){
+     r <@ A.run1();
+   }else{
+     r' <@ A.run2();
+     r  <- !r;
+   }
+   return r;
+  }
+
+
+}.
+
+end section.
+
+section.
+
+declare module A <: IR1R2.
+
+op f (x : real) : real = 1%r/2%r * (1%r + x).
+op fop (x : real) : real = 2%r * x - 1%r.
+
+lemma f_pr1 (a b : real) : a <= b => f a <= f b.
+smt.
+qed.
+
+
+lemma f_pr2 (a b : real) : f a <= f b => a <= b.
+smt.
+qed.
+
+lemma f_pr3 (a  : real) : f (fop a) = a.
+smt.
+qed.
+
+lemma f_pr4 (a  : real) : fop (f a) = a.
+smt.
+qed.
+
+
+lemma f_pr5 (a b : real) : a <= b => fop a <= fop b.
+smt.
+qed.
+
+lemma f_pr6 (a b : real) : fop a <= fop b =>  a <= b.
+smt.
+qed.
+
+
+
+lemma d_b1 &m : Pr[ P(A).init_main12() @ &m : res ] 
+  = f (Pr[ P(A).main1() @ &m : res ] - Pr[ P(A).main2() @ &m : res ]) .
+admitted.
+
+lemma d_b2 &m : Pr[ P(A).main12() @ &m : res ] 
+  = f (Pr[ A.run1() @ &m : res ] - Pr[ A.run2() @ &m : res ]) .
+admitted.
+
+
+lemma d_b3 &m p : p >= Pr[ P(A).init_main12() @ &m : res ] 
+   => exists &n, p >= Pr[ P(A).main12() @ &n : res ].
+admitted.
+
+
+lemma o_0 &m p: 
+       p >=  Pr[ P(A).main1() @ &m : res ]  - 
+               Pr[ P(A).main2() @ &m : res ]
+   => exists &n, p >= Pr[ A.run1() @ &n : res ] - Pr[ A.run2() @ &n : res ].
+progress.
+have f1 : Pr[P(A).main1() @ &m : res] - Pr[P(A).main2() @ &m : res]
+  = fop (Pr[ P(A).init_main12() @ &m : res ] ).
+rewrite d_b1. smt.
+have f2 : p >= fop Pr[P(A).init_main12() @ &m : res].
+smt.
+have f3 : f p >= Pr[P(A).init_main12() @ &m : res]. smt.
+have f4 : exists &n,  f p >= Pr[ P(A).main12() @ &n : res ].
+apply (d_b3 &m (f p)). auto.
+elim f4. progress.
+exists &n.
+smt.
+qed.
+  
+
+
+   
+end section.
